finished the new version of SpecM.v with SpecDefs

theories/Ref/SpecM.v
@@ -121,6 +121,19 @@ Proof.
   unfold pcons_r. rewrite papp_assoc. reflexivity.
 Qed.
 
+Polymorphic Fixpoint papp_r@{u} {A : Type@{u}} (xs ys : plist A) : plist A :=
+  match ys with
+  | pnil => xs
+  | pcons y ys' => papp_r (pcons_r xs y) ys'
+  end.
+
+Lemma papp_r_papp {A} (xs ys : plist A) : papp_r xs ys = papp xs ys.
+Proof.
+  revert xs; induction ys; intros.
+  - symmetry. apply papp_nil.
+  - simpl. rewrite IHys. apply pcons_r_app.
+Qed.
+
 (* FIXME: doesn't work!
 Polymorphic Fixpoint pconcat@{u} {A : Type@{u}} (xss : plist (plist A)) : plist A :=
   match xss with
@@ -700,13 +713,13 @@ Definition importInclImp E (imp : SpecDef E) stk stk_def :
 (* Build a stack inclusion for the defined spec in importSpecDef *)
 Definition importInclDef E (imp : SpecDef E) stk stk_def :
   stackIncl
-    (papp (pcons (relDefOut _ _ imp) stk) stk_def)
+    (papp (pcons_r stk (relDefOut _ _ imp)) stk_def)
     (papp stk (papp (relDefStack _ _ imp) stk_def)).
 Admitted.
 
 (* Import a SpecDef into another, by allowing the latter to call the former *)
 Program Definition importSpecDef E (imp : SpecDef E) stk
-  (d : RelSpecDef E (pcons (relDefOut E pnil imp) stk)) :
+  (d : RelSpecDef E (pcons_r stk (relDefOut E pnil imp))) :
   RelSpecDef E stk :=
   {|
     relDefStack := papp (relDefStack _ _ imp) (relDefStack _ _ d);
@@ -732,81 +745,29 @@ Next Obligation.
 Defined.
 
 
-
-
-(* Build a SpecDef from a tuple of defs that can call into each other and into
-any of a list of sub-definitions *)
-Definition defineSpec E (imps : plist (SpecDef E)) (lrts : plist LetRecType)
-  (defs : PolyFrameTuple E (papp lrts (pmap (SpecDefOut E) subDefs)) lrts)
-  (n : nat) (lt : n < plength lrts) : SpecDef E :=
-  {|
-    SpecDef_stack := papp lrts (pconcat (pmap (SpecDef_stack E) subDefs));
-    SpecDef_bodies :=
-      fun stack' incl =>
-    SpecDef_call := n; |}.
-
-
-
-
-FIXME: old stuff below
-
-(* A SpecDef represents a definition of a SpecM monadic function via MultiFixsS
-as a FrameTuple plus an index into that FrameTuple *)
-Record SpecDef E :=
-  { SpecDef_stack : FunStack;
-    SpecDef_bodies : PolyFrameTuple E SpecDef_stack SpecDef_stack;
-    SpecDef_call : nat;
-    SpecDef_callLt : SpecDef_call < plength SpecDef_stack }.
-
-(* The output type of the main definition of a SpecDef *)
-Definition SpecDefOut E (d : SpecDef E) : LetRecType :=
-  nthLRT (SpecDef_stack _ d) (SpecDef_call _ d).
-
-(* Build a stackIncl from  *)
-Fixpoint inclSpecDefCalls E (ds : plist (SpecDef E)) :
-  stackIncl (pmap (SpecDefOut E) ds) (pconcat (pmap (SpecDef_stack E) ds)) :=
-  match ds return stackIncl (pmap (SpecDefOut E) ds)
-                    (pconcat (pmap (SpecDef_stack E) ds)) with
-  | pnil => reflStackIncl pnil
-  | pcons d ds' =>
-      consPrefixStackIncl
-        (SpecDef_call E d) (SpecDef_stack E d) (SpecDef_callLt E d) _ _
-        (inclSpecDefCalls E ds')
+Fixpoint defineRelSpec E stk (imps : plist (SpecDef E)) :
+  RelSpecDef E (papp_r stk (pmap (relDefOut _ _) imps)) -> RelSpecDef E stk :=
+  match imps return RelSpecDef E (papp_r stk (pmap (relDefOut _ _) imps)) ->
+                    RelSpecDef E stk with
+  | pnil => fun d => d
+  | pcons imp imps' =>
+      fun d =>
+        importSpecDef E imp stk (defineRelSpec E _ imps' d)
   end.
 
-(*
-(* Call the nth recursive function in a SpecM computation *)
-Definition callNth E stack n :
-  lrtPi stack (nthLRT stack n) (fun args => SpecM E stack (LRTOutput _ _ args)) :=
-  lrtLambda
-    stack (nthLRT stack n)
-    (fun args => SpecM E stack (LRTOutput _ _ args))
-    (fun args => trigger args).
+Program Definition castRelSpecDef E stk1 stk2 (e : stk1 = stk2)
+  (d : RelSpecDef E stk1) : RelSpecDef E stk2 := d.
 
-Definition callNthCast E stack n lrt (e : nthLRT stack n = lrt) :
-  lrtPi stack lrt (fun args => SpecM E stack (LRTOutput _ _ args)) :=
-  eq_rect (nthLRT stack n)
-    (fun lrt' => lrtPi stack lrt' (fun args => SpecM E stack (LRTOutput _ _ args)))
-    (callNth E stack n)
-    lrt e.
-*)
-
-(* Build a SpecDef from a tuple of defs that can call into each other and into
-any of a list of sub-definitions *)
-Definition defineSpec E (subDefs : plist (SpecDef E)) (lrts : plist LetRecType)
-  (defs : PolyFrameTuple E (papp lrts (pmap (SpecDefOut E) subDefs)) lrts)
-  (n : nat) : SpecDef E :=
-  {|
-    SpecDef_stack := papp lrts (pconcat (pmap (SpecDef_stack E) subDefs));
-    SpecDef_bodies :=
-      fun stack' incl =>
-    SpecDef_call := n; |}.
+Program Definition defineSpec E (imps : plist (SpecDef E))
+                      (d : RelSpecDef E (pmap (relDefOut _ _) imps)) : SpecDef E :=
+  defineRelSpec _ _ imps (castRelSpecDef _ _ _ _ d).
+Next Obligation.
+  rewrite papp_r_papp. reflexivity.
+Defined.
 
 
-FIXME HERE: maybe we don't need LRTValue and friends?
-
+(* FIXME: just keeping LRTValue in case it is useful in the future...
 (* A value of an LRTArgType *)
-(* FIXME: figure out how to define MultiFixS using this LRTValueFun type... *)
 Fixpoint LRTValue E (stack:FunStack) (argTp : LRTArgType) : Type@{entree_u} :=
   match argTp with
   | ArgType_Const A => A
@@ -855,625 +816,7 @@ LRTArgFun2ValueFun E stack lrt : (forall args:LRTInput stack lrt,
       fun f a =>
         LRTArgFun2ValueFun E stack lrt' (fun args => f (a, args))
   end.
-
-FIXME: old stuff below
-
-(* An element of an LRTArgType, which is either a decoding of the LRTArgType to
-an actual Coq type or a recursive call of the given type in the frame *)
-Fixpoint LRTArgTypeElem (M : Type@{entree_u} -> Type@{entree_u})
-  (argTp : LRTArgType) : Type@{entree_u} :=
-  match argTp with
-  | ArgType_Const A => A
-  | ArgType_Prod A B => LRTArgTypeElem M A * LRTArgTypeElem M B
-  | ArgType_Sigma A B => { x:A & LRTArgTypeElem M (B x) }
-  | ArgType_Arrow A B => LRTArgTypeElem M A -> LRTArgTypeElem M B
-  | ArgType_Pi A B => forall x:A, LRTArgTypeElem M (B x)
-  | ArgType_M A => M (LRTArgTypeElem M A)
-  end.
-
-(* The type of a recursive function *)
-Inductive LetRecType : Type@{entree_u + 1} :=
-| LRT_Ret (R : LRTArgType) : LetRecType
-| LRT_FunDep (A : Type@{entree_u}) (rest : A -> LetRecType) : LetRecType
-| LRT_Fun (A : LRTArgType) (rest : LetRecType) : LetRecType
-.
-
-(* Compute a dependent tuple type of all the inputs of a LetRecType, i.e.,
-   return the type { x:A & { y:B & ... { z:C & unit } ...}} from a LetRecType
-   that represents forall a b c..., SpecM ... (R a b c ...). The supplied type
-   function M gives the interpretation of the ArgType_M type constructor. *)
-Fixpoint LRTInput (M : Type@{entree_u} -> Type@{entree_u}) lrt : Type@{entree_u} :=
-  match lrt with
-  | LRT_Ret _ => unit
-  | LRT_FunDep A rest => {a : A & LRTInput M (rest a) }
-  | LRT_Fun A rest => LRTArgTypeElem M A * LRTInput M rest
-  end.
-
-(* Compute the output type (R a b c ...) from a LetRecType that represents
-   forall a b c..., SpecM ... (R a b c ...) and a dependent tuple of arguments
-   to a function of that type, using M for the ArgType_M type constructor *)
-Fixpoint LRTOutput M lrt : EncodingType (LRTInput M lrt) :=
-  match lrt with
-  | LRT_Ret R => fun _ => LRTArgTypeElem M R
-  | LRT_FunDep A rest => fun args =>
-                           let '(existT _ a args') := args in
-                           LRTOutput M (rest a) args'
-  | LRT_Fun A rest => fun args => LRTOutput M rest (snd args)
-  end.
-
-(* Build the type forall a b c ..., F (a, (b, (c, ...))) for an arbitrary type
-   function F over an LRTInput *)
-Fixpoint lrtPi M lrt : (LRTInput M lrt -> Type) -> Type :=
-  match lrt return (LRTInput M lrt -> Type) -> Type with
-  | LRT_Ret _ => fun F => F tt
-  | LRT_FunDep A lrtF =>
-      fun F => forall a, lrtPi M (lrtF a) (fun args => F (existT _ a args))
-  | LRT_Fun A lrt' =>
-      fun F => forall a, lrtPi M lrt' (fun args => F (a, args))
-  end.
-
-(* Build an lrtPi function from a unary function on an LRTInput *)
-Fixpoint lrtLambda M lrt
-  : forall (F : LRTInput M lrt -> Type), (forall args, F args) -> lrtPi M lrt F :=
-  match lrt return forall (F : LRTInput M lrt -> Type), (forall args, F args) ->
-                                                        lrtPi M lrt F
-  with
-  | LRT_Ret _ => fun _ f => f tt
-  | LRT_FunDep A lrtF =>
-    fun F f a => lrtLambda M (lrtF a)
-                   (fun args => F (existT _ a args))
-                   (fun args => f (existT _ a args))
-  | LRT_Fun A lrt' =>
-      fun F f a => lrtLambda M lrt'
-                     (fun args => F (a, args))
-                     (fun args => f (a, args))
-  end.
-
-(* Apply an lrtPi function *)
-Fixpoint lrtApply M lrt
-  : forall F, lrtPi M lrt F -> forall args, F args :=
-  match lrt return forall F, lrtPi M lrt F -> forall args, F args with
-  | LRT_Ret _ =>
-    fun F f u => match u return F u with | tt => f end
-  | LRT_FunDep A lrtF =>
-    fun F f args =>
-      match args return F args with
-      | existT _ arg args' =>
-        lrtApply M (lrtF arg) (fun args' => F (existT _ arg args')) (f arg) args'
-      end
-  | LRT_Fun A lrt' =>
-    fun F f args =>
-      match args return F args with
-      | (arg, args') =>
-        lrtApply M lrt' (fun args' => F (arg, args')) (f arg) args'
-      end
-  end.
-
-(* NOTE: it is straightforward to prove a beta rule for lrtApply lrtLambda, but
-   that isn't really needed below *)
-
-
-(** Frames, FrameCalls, and FunStackE **)
-
-(* A recursive function frame is specified by a list of LetRecTypes *)
-Definition RecFrame := list LetRecType.
-
-(* Get the nth element of a RecFrame list, or void -> void if n is too big *)
-Definition nthLRT (frame : RecFrame) n : LetRecType :=
-  nth_default' (LRT_Fun (ArgType_Const void) (LRT_Ret (ArgType_Const void))) frame n.
-
-(* A recursive call to one of the functions in a RecFrame, specified by a
-natural number n that picks a specific index in the RecFrame along with a set of
-arguments for that recursive call, using the given type function M as the
-interpretation of the ArgType_M constructor *)
-Inductive FrameCallH M frame : Type@{entree_u} :=
-| FrameCallOfArgs n (args : LRTInput M (nthLRT frame n)).
-
-(* The return type for a FrameCallH recursive call, using a specific M *)
-Definition FrameCallHRet M frame (args: FrameCallH M frame) : Type@{entree_u} :=
-  match args with
-  | FrameCallOfArgs _ _ n args => LRTOutput M (nthLRT frame n) args
-  end.
-
-(* The type of a FrameCallH recursive call along with a FrameCallHRet function
-that computes the return type of one of those recursive calls, but where the
-arguments to the recursive call are at a specified "level". A level 0 frame call
-is one whose higher-order arguments can only contain calls to monadic functions
-of return type M0, while a level S lvl' call can contain higher-order arguments
-with frame calls at level lvl' or below. *)
-Fixpoint FrameCallLvlInOut (M0 : Type@{entree_u} -> Type@{entree_u}) frame lvl
-  : EncType@{entree_u} :=
-  match lvl with
-  | 0 => Build_EncType (FrameCallH M0 frame) (FrameCallHRet M0 frame)
-  | S lvl' =>
-      let M := fun R =>
-                 (M0 R +
-                    { args:FrameCallLvlInOut M0 frame lvl'
-                    | encodes args = R })%type in
-      Build_EncType (FrameCallH M frame) (FrameCallHRet M frame)
-  end.
-
-(* A frame call at an arbitrary level, where M0 defines level 0 *)
-Definition FrameCall (M0 : Type@{entree_u} -> Type@{entree_u}) frame :=
-  { lvl & FrameCallLvlInOut M0 frame lvl }.
-
-(* Compute the return type of a FrameCall *)
-Definition FrameCallRet (M0 : Type@{entree_u} -> Type@{entree_u}) frame
-                        (call : FrameCall M0 frame) : Type@{entree_u} :=
-  encodes (projT2 call).
-
-Global Instance EncodingType_FrameCall M0 frame : EncodingType (FrameCall M0 frame) :=
-  FrameCallRet M0 frame.
-
-
-(* A FunStack is a list of RecFrame representing all of the functions bound
-    by multiFixS that are currently in scope *)
-Definition FunStack := list RecFrame.
-
-(* The error event type *)
-Inductive ErrorE : Set :=
-| mkErrorE : string -> ErrorE.
-
-Global Instance EncodingType_ErrorE : EncodingType ErrorE := fun _ => void.
-
-(* Create an event type for either an event in E or a recursive call in a stack
-   Γ of recursive functions in scope *)
-Fixpoint FunStackE (E : Type) `{EncodingType E} (stack : FunStack) : EncType@{entree_u} :=
-  match stack with
-  | nil => Build_EncType (ErrorE + E) _
-  | frame :: stack' =>
-      let M := fun R => entree_spec (FunStackE E stack') R in
-      Build_EncType (FrameCall M frame + FunStackE E stack') _
-  end.
-
-(* Embed an underlying event into the FunStackE event type *)
-Fixpoint FunStackE_embed_ev (E : Type) `{EncodingType E} Γ (e : ErrorE + E) : FunStackE E Γ :=
-  match Γ return FunStackE E Γ with
-  | nil => e
-  | (_ :: Γ') => inr (FunStackE_embed_ev E Γ' e)
-  end.
-
-(* Map the output of a FunStackE event for an E to the output type of E *)
-Fixpoint FunStackE_embed_ev_unmap (E : Type) `{EncodingType E} Γ e
-  : encodes (FunStackE_embed_ev E Γ e) -> encodes e :=
-  match Γ return encodes (FunStackE_embed_ev E Γ e) -> encodes e with
-  | nil => fun o => o
-  | (_ :: Γ') => FunStackE_embed_ev_unmap E Γ' e
-  end.
-
-Global Instance ReSum_FunStackE_E (E : Type) `{EncodingType E} (Γ : FunStack) : ReSum E (FunStackE E Γ) :=
-  fun e => FunStackE_embed_ev E Γ (inr e).
-
-Global Instance ReSumRet_FunStackE_E (E : Type) `{EncodingType E} Γ :
-  ReSumRet E (FunStackE E Γ) :=
-  fun e => FunStackE_embed_ev_unmap E Γ (inr e).
-
-Global Instance ReSum_FunStackE_Error (E : Type) `{EncodingType E} (Γ : FunStack) : ReSum ErrorE (FunStackE E Γ) :=
-  fun e => FunStackE_embed_ev E Γ (inl e).
-
-Global Instance ReSumRet_FunStackE_Error (E : Type) `{EncodingType E} Γ :
-  ReSumRet ErrorE (FunStackE E Γ) :=
-  fun e => FunStackE_embed_ev_unmap E Γ (inl e).
-
-Global Instance ReSum_cons_FunStack E `{EncodingType E} (stack : FunStack) frame :
-  ReSum (SpecEvent (FunStackE E stack)) (SpecEvent (FunStackE E (frame :: stack))) :=
-  fun e => match e with
-           | Spec_vis e => Spec_vis (resum e)
-           | Spec_forall T => Spec_forall T
-           | Spec_exists T => Spec_exists T
-           end.
-
-Global Instance ReSumRet_nil_FunStack E `{EncodingType E} stack frame :
-  ReSumRet (SpecEvent (FunStackE E stack)) (SpecEvent (FunStackE E (frame :: stack))) :=
-  fun e =>
-    match e return encodes (ReSum_cons_FunStack E stack frame e) -> encodes e with
-    | Spec_vis e => fun x => resum_ret e x
-    | Spec_forall T => fun x => x
-    | Spec_exists T => fun x => x
-    end.
-
-
-(** The SpecM monad and associated operations **)
-
-(* The SpecM monad is the entree_spec monad with FunStackE as the event type *)
-Definition SpecM (E:EncType) stack A : Type@{entree_u} :=
-  entree_spec (FunStackE E stack) A.
-
-Definition RetS {E} {Γ A} (a : A) : SpecM E Γ A := ret a.
-Definition BindS {E} {Γ A B} (m : SpecM E Γ A) (k : A -> SpecM E Γ B) :=
-  bind m k.
-Definition IterS {E} {Γ A B} (body : A -> SpecM E Γ (A + B)) :
-  A -> SpecM E Γ B := EnTree.iter body.
-Definition AssumeS {E} {Γ} (P : Prop) : SpecM E Γ unit :=
-  assume_spec P.
-Definition AssertS {E} {Γ} (P : Prop) : SpecM E Γ unit :=
-  assert_spec P.
-Definition ForallS {E} {Γ} (A : Type) `{QuantType A} : SpecM E Γ A :=
-  forall_spec A.
-Definition ExistsS {E} {Γ} (A : Type) `{QuantType A} : SpecM E Γ A :=
-  exists_spec A.
-Definition TriggerS {E:EncType} {Γ} (e : E) : SpecM E Γ (encodes e) := trigger e.
-Definition ErrorS {E} {Γ} A (str : string) : SpecM E Γ A :=
-  bind (trigger (mkErrorE str)) (fun (x:void) => match x with end).
-
-Global Instance SpecM_Monad {E} Γ : Monad (SpecM E Γ) :=
-  {|
-    ret := fun A a => RetS a;
-    bind := fun A B m k => BindS m k;
-  |}.
-
-(* Cons a frame onto the stack of a SpecM computation *)
-Definition consStackS E stack frame A (t:SpecM E stack A) : SpecM E (frame :: stack) A :=
-  resumEntree t.
-
-
-(** Making recursive calls **)
-
-(* A FrameCall that calls into the topmost frame *)
-Definition TopFrameCall (E:EncType) stack frame :=
-  FrameCall (SpecM E stack) frame.
-
-(* The return type of a TopFrameCall *)
-Definition TopFrameCallRet (E:EncType) stack frame
-  : TopFrameCall E stack frame -> Type :=
-  FrameCallRet (SpecM E stack) frame.
-
-(* Create a recursive call to a function in the top-most frame using args *)
-Definition CallS E stack frame (args : TopFrameCall E stack frame) :
-  SpecM E (frame :: stack) (TopFrameCallRet E stack frame args) :=
-  trigger args.
-
-FIXME HERE: how to define mkTopFrameCall to take in arguments which can have recursive calls to the same top frame?
-
-(* Make a TopFrameCall from its individual arguments *)
-Definition mkTopFrameCall E stack frame n
-  : lrtPi (SpecM E stack) (nthLRT frame n) (fun args => TopFrameCall E stack frame) :=
-  lrtLambda (SpecM E stack) (nthLRT frame n) (fun _ => TopFrameCall E stack frame) (FrameCallOfArgs _ frame n).
-
-
-FIXME: update the below
-
-(* Add a function type to the frame of a FrameCall *)
-Definition consFrameCall {lrt frame} (call : FrameCall frame)
-  : FrameCall (cons lrt frame) :=
-  match call in FrameCall _ return FrameCall (cons lrt frame) with
-  | FrameCallOfArgs _ n args => FrameCallOfArgs (cons lrt frame) (S n) args
-  end.
-
-(* The index of a FrameCall is always less than the length of the frame *)
-Lemma FrameCallIndexLt frame call : @FrameCallIndex frame call < length frame.
-Proof.
-  destruct call.
-  revert frame args; induction n; intros; destruct frame;
-    try (destruct args; destruct x).
-  - simpl. apply Lt.neq_0_lt. trivial.
-  - simpl. apply Lt.lt_n_S. apply (IHn _ args).
-Qed.
-
-(* The return type for calling a recursive function in a RecFrame *)
-Definition FrameCallRet frame (args: FrameCall frame) : Type@{entree_u} :=
-  match args with
-  | FrameCallOfArgs _ n args => LRTOutput (nthLRT frame n) args
-  end.
-
-Global Instance FrameCallRetEncoding lrt : EncodingType (FrameCall lrt) :=
-  FrameCallRet lrt.
-
-(* Make a recursive call from its individual arguments *)
-Definition mkFrameCall (frame : RecFrame) n
-  : lrtPi (nthLRT frame n) (fun args => FrameCall frame) :=
-  lrtLambda (nthLRT frame n) (fun _ => FrameCall frame) (FrameCallOfArgs frame n).
-
-(* ReSum instances for embedding the nth LRTInput into a FrameCall *)
-Global Instance FrameCall_ReSum frame n :
-  ReSum (LRTInput (nthLRT frame n)) (FrameCall frame) := FrameCallOfArgs frame n.
-Global Instance FrameCall_ReSumRet frame n :
-  ReSumRet (LRTInput (nthLRT frame n)) (FrameCall frame) :=
-  fun _ r => r.
-
-(* A FunStack is a list of RecFrame representing all of the functions bound
-    by multiFixS that are currently in scope *)
-Definition FunStack := list RecFrame.
-
-(* The error event type *)
-Inductive ErrorE : Set :=
-| mkErrorE : string -> ErrorE.
-
-Global Instance EncodingType_ErrorE : EncodingType ErrorE := fun _ => void.
-
-(* Create an event type for either an event in E or a recursive call in a stack
-   Γ of recursive functions in scope *)
-Fixpoint FunStackE (E : Type) (Γ : FunStack) : Type@{entree_u} :=
-  match Γ with
-  | nil => ErrorE + E
-  | frame :: Γ' => FrameCall frame + FunStackE E Γ'
-  end.
-
-(* Compute the output type for a FunStackE event *)
-Fixpoint FunStackE_encodes (E : Type) `{EncodingType E} (Γ : FunStack) :
-  FunStackE E Γ -> Type@{entree_u} :=
-  match Γ return FunStackE E Γ -> Type with
-  | nil => fun e => encodes e
-  | frame :: Γ' => fun e => match e with
-                            | inl args => FrameCallRet frame args
-                            | inr args => FunStackE_encodes E Γ' args
-                            end
-  end.
-
-Global Instance FunStackE_encodes' (E : Type) `{EncodingType E} (Γ : FunStack) : EncodingType (FunStackE E Γ) :=
-  FunStackE_encodes E Γ.
-
-(* Embed an underlying event into the FunStackE event type *)
-Fixpoint FunStackE_embed_ev (E : Type) Γ (e : ErrorE + E) : FunStackE E Γ :=
-  match Γ return FunStackE E Γ with
-  | nil => e
-  | (_ :: Γ') => inr (FunStackE_embed_ev E Γ' e)
-  end.
-
-(* Map the output of a FunStackE event for an E to the output type of E *)
-Fixpoint FunStackE_embed_ev_unmap (E : Type) `{EncodingType E} Γ e
-  : encodes (FunStackE_embed_ev E Γ e) -> encodes e :=
-  match Γ return encodes (FunStackE_embed_ev E Γ e) -> encodes e with
-  | nil => fun o => o
-  | (_ :: Γ') => FunStackE_embed_ev_unmap E Γ' e
-  end.
-
-Global Instance ReSum_FunStackE_E (E : Type) (Γ : FunStack) : ReSum E (FunStackE E Γ) :=
-  fun e => FunStackE_embed_ev E Γ (inr e).
-
-Global Instance ReSumRet_FunStackE_E (E : Type) `{EncodingType E} Γ :
-  ReSumRet E (FunStackE E Γ) :=
-  fun e => FunStackE_embed_ev_unmap E Γ (inr e).
-
-Global Instance ReSum_FunStackE_Error (E : Type) (Γ : FunStack) : ReSum ErrorE (FunStackE E Γ) :=
-  fun e => FunStackE_embed_ev E Γ (inl e).
-
-Global Instance ReSumRet_FunStackE_Error (E : Type) `{EncodingType E} Γ :
-  ReSumRet ErrorE (FunStackE E Γ) :=
-  fun e => FunStackE_embed_ev_unmap E Γ (inl e).
-
-(* Get the nth RecFrame frame in a FunStack, returning the empty frame if n
-   is too big *)
-Definition nthFrame (Γ : FunStack) fnum : RecFrame :=
-  nth_default' nil Γ fnum.
-
-(* Embed a FrameCall for the fnum-th frame of a FunStack into FunStackE *)
-(*
-Fixpoint mkFunStackE E Γ fnum : FrameCall (nthFrame Γ fnum) -> FunStackE E Γ :=
-  match Γ return FrameCall (nthFrame Γ fnum) -> FunStackE E Γ with
-  | nil => fun x => match x with end
-  | frame :: Γ' =>
-    match fnum return FrameCall (nthFrame (frame :: Γ') fnum) ->
-                      FunStackE E (frame :: Γ') with
-    | 0 => fun args => inl args
-    | S fnum' => fun args => inr (mkFunStackE E Γ' fnum' args)
-    end
-  end.
-
-(* Embed an LRTInput for the nth function in the fnum-th frame of a FunStack
-   into FunStackE *)
-Definition mkFunStackE' E Γ fnum n
-           (args:LRTInput (nthLRT (nthFrame Γ fnum) n)) : FunStackE E Γ :=
-  mkFunStackE E Γ fnum (embedFrameCall _ n args).
 *)
-
-(* Embed a call in the top level of the FunStack into a FunStackE *)
-Global Instance ReSum_LRTInput_FunStackE (E : Type) (Γ : FunStack) frame n :
-  ReSum (LRTInput (nthLRT frame n)) (FunStackE E (frame :: Γ)) :=
-  fun args => inl (FrameCallOfArgs frame n args).
-
-(* Map the return value for embedding a call in the top level to a FunStackE *)
-Global Instance ReSumRet_LRTInput_FunStackE (E : Type) `{EncodingType E} Γ frame n
-  : ReSumRet (LRTInput (nthLRT frame n)) (FunStackE E (frame :: Γ)) :=
-  fun args o => o.
-
-(* Embed a call in the top level of the FunStack into a FunStackE *)
-Global Instance ReSum_FrameCall_FunStackE (E : Type) (Γ : FunStack) frame :
-  ReSum (FrameCall frame) (FunStackE E (frame :: Γ)) :=
-  fun args => inl args.
-
-(* Map the return value for embedding a call in the top level to a FunStackE *)
-Global Instance ReSumRet_FrameCall_FunStackE (E : Type) `{EncodingType E} Γ frame :
-  ReSumRet (FrameCall frame) (FunStackE E (frame :: Γ)) :=
-  fun args o => o.
-
-
-(* An EvType is an event type E plus a return type for each event in E *)
-Record EvType : Type :=
-  { evTypeType :> Type@{entree_u};
-    evRetType : evTypeType -> Type@{entree_u} }.
-
-Global Instance EncodingType_EvType (E:EvType) : EncodingType E :=
-  fun e => evRetType E e.
-
-Global Instance ReSum_FunStack_EvType (E : EvType) Γ : ReSum E (FunStackE E Γ) :=
-  ReSum_FunStackE_E _ _.
-Global Instance ReSumRet_FunStack_EvType (E : EvType) Γ : ReSumRet E (FunStackE E Γ) :=
-  ReSumRet_FunStackE_E _ _.
-
-(* The SpecM monad is the entree_spec monad with FunStackE as the event type *)
-Definition SpecM (E:EvType) Γ A : Type@{entree_u} :=
-  entree_spec (FunStackE E Γ) A.
-
-Definition RetS {E} {Γ A} (a : A) : SpecM E Γ A := ret a.
-Definition BindS {E} {Γ A B} (m : SpecM E Γ A) (k : A -> SpecM E Γ B) :=
-  bind m k.
-Definition IterS {E} {Γ A B} (body : A -> SpecM E Γ (A + B)) :
-  A -> SpecM E Γ B := EnTree.iter body.
-Definition AssumeS {E} {Γ} (P : Prop) : SpecM E Γ unit :=
-  assume_spec P.
-Definition AssertS {E} {Γ} (P : Prop) : SpecM E Γ unit :=
-  assert_spec P.
-Definition ForallS {E} {Γ} (A : Type) `{QuantType A} : SpecM E Γ A :=
-  forall_spec A.
-Definition ExistsS {E} {Γ} (A : Type) `{QuantType A} : SpecM E Γ A :=
-  exists_spec A.
-Definition TriggerS {E:EvType} {Γ} (e : E) : SpecM E Γ (encodes e) := trigger e.
-Definition ErrorS {E} {Γ} A (str : string) : SpecM E Γ A :=
-  bind (trigger (mkErrorE str)) (fun (x:void) => match x with end).
-
-Global Instance SpecM_Monad {E} Γ : Monad (SpecM E Γ) :=
-  {|
-    ret := fun A a => RetS a;
-    bind := fun A B m k => BindS m k;
-  |}.
-
-Global Instance ReSum_nil_FunStack E (Γ : FunStack) :
-  ReSum (SpecEvent (FunStackE E nil)) (SpecEvent (FunStackE E Γ)) :=
-  fun e => match e with
-           | Spec_vis (inl el) => Spec_vis (resum el)
-           | Spec_vis (inr er) => Spec_vis (resum er)
-           | Spec_forall T => Spec_forall T
-           | Spec_exists T => Spec_exists T
-           end.
-
-Global Instance ReSumRet_nil_FunStack (E:EvType) (Γ : FunStack) :
-  ReSumRet (SpecEvent (FunStackE E nil)) (SpecEvent (FunStackE E Γ)) :=
-  fun e =>
-    match e return encodes (ReSum_nil_FunStack E Γ e) -> encodes e with
-    | Spec_vis (inl el) => fun x => resum_ret el x
-    | Spec_vis (inr er) => fun x => resum_ret er x
-    | Spec_forall T => fun x => x
-    | Spec_exists T => fun x => x
-    end.
-
-
-(* Lift a SpecM in the empty FunStack to an arbitrary FunStack *)
-Definition liftStackS {E} {Γ} A (t:SpecM E nil A) : SpecM E Γ A :=
-  resumEntree t.
-
-(* Compute the type forall a b c ... . SpecM ... (R a b c ...) from an lrt *)
-(*
-Fixpoint LRTType E `{EncodingType E} Γ (lrt : LetRecType) : Type@{entree_u} :=
-  match lrt with
-  | LRT_Ret R => SpecM E Γ R
-  | LRT_Fun A rest => forall (a : A), LRTType E Γ (rest a)
-  end.
-*)
-Definition LRTType E Γ lrt : Type@{entree_u} :=
-  lrtPi lrt (fun args => SpecM E Γ (LRTOutput lrt args)).
-
-(* Create a recursive call to a function in the top-most using args *)
-Definition CallS E Γ frame (args : FrameCall frame) :
-  SpecM E (frame :: Γ) (FrameCallRet frame args) :=
-  trigger (H2:=@SpecEventReSumRet _ _ _ _ _ _) args.
-
-(* Build the right-nested tuple type of a list of functions in a RecFrame *)
-Fixpoint FrameTuple E Γ (frame : RecFrame) : Type@{entree_u} :=
-  match frame with
-  | nil => unit
-  | lrt :: frame' => LRTType E Γ lrt * FrameTuple E Γ frame'
-  end.
-
-(* Get the nth function in a FrameTuple *)
-Fixpoint nthFrameTupleFun E Γ frame : forall n, FrameTuple E Γ frame ->
-                                                LRTType E Γ (nthLRT frame n) :=
-  match frame return forall n, FrameTuple E Γ frame ->
-                               LRTType E Γ (nthLRT frame n) with
-  | nil => fun _ _ v => match v with end
-  | lrt :: frame' =>
-    fun n => match n return FrameTuple E Γ (lrt :: frame') ->
-                            LRTType E Γ (nthLRT (lrt :: frame') n) with
-             | 0 => fun tup => fst tup
-             | S n' => fun tup => nthFrameTupleFun E Γ frame' n' (snd tup)
-             end
-  end.
-
-(* Apply a FrameTuple to a FrameCall to get a FrameCallRet *)
-Definition applyFrameTuple E Γ frame (funs : FrameTuple E Γ frame)
-           (call : FrameCall frame) : SpecM E Γ (FrameCallRet frame call) :=
-  match call return SpecM E Γ (FrameCallRet frame call) with
-  | FrameCallOfArgs _ n args =>
-    lrtApply (nthLRT frame n) _ (nthFrameTupleFun _ _ frame n funs) args
-  end.
-
-(* Create a multi-way fixed point of a sequence of functions *)
-Definition MultiFixS E Γ frame
-           (bodies : FrameTuple E (frame :: Γ) frame)
-           (call : FrameCall frame) : SpecM E Γ (FrameCallRet frame call) :=
-  mrec_spec (applyFrameTuple E (frame :: Γ) frame bodies) call.
-
-
-
-FIXME: old stuff below
-
-(** Stack functors and using them in MultiFixS **)
-
-(* A StackType is a type that depends on a FunStack *)
-Definition StackType := FunStack -> Type@{entree_u}.
-
-(* A stack functor is a type which depends on the current FunStack that supports
-pushing and popping the FunStack as long as we have an interpretation of each
-frame that is pushed or popped *)
-Class IsStackFunc E (T : StackType) :=
-  { pushSF : forall Γ frame,
-      FrameTuple E (frame :: Γ) frame ->
-      T Γ -> T (frame :: Γ);
-    popSF : forall Γ frame,
-      FrameTuple E (frame :: Γ) frame ->
-      T (frame :: Γ) -> T Γ; }.
-
-Definition constST T : StackType := fun _ => T.
-
-#[global] Instance IsStackFunc_const E T : IsStackFunc E (constST T) :=
-  { pushSF := fun _ _ _ x => x; popSF := fun _ _ _ x => x }.
-
-Definition prodST (T1 T2 : StackType) : StackType :=
-  (fun stk => prod (T1 stk) (T2 stk)).
-
-#[global] Instance IsStackFunc_pair E T1 T2
-  {isSF1 : IsStackFunc E T1} {isSF2 : IsStackFunc E T2} :
-  IsStackFunc E (prodST T1 T2) :=
-  { pushSF := fun stk frame interp tup => (pushSF stk frame interp (fst tup),
-                                            pushSF stk frame interp (snd tup));
-    popSF := fun stk frame interp tup => (popSF stk frame interp (fst tup),
-                                           popSF stk frame interp (snd tup)); }.
-
-Definition arrowST (T U : StackType) : StackType :=
-  fun stk => T stk -> U stk.
-
-#[global] Instance IsStackFunc_fun E T1 T2 
-  {isSF1 : IsStackFunc E T1} {isSF2 : IsStackFunc E T2} :
-  IsStackFunc E (arrowST T1 T2) :=
-  { pushSF := fun stk frame interp f x =>
-                pushSF stk frame interp (f (popSF stk frame interp x));
-    popSF := fun stk frame interp f x =>
-               popSF stk frame interp (f (pushSF stk frame interp x)); }.
-
-(* A variant of LetRecType where arguments and the return type can depend on the
-current stack, though arguments that do are not allowed to be type indices *)
-Inductive LetRecTypeSF E : Type@{entree_u + 1} :=
-| LRTSF_Ret R `{IsStackFunc E R} : LetRecTypeSF E
-| LRTSF_Fun (A : Type@{entree_u}) (rest : A -> LetRecTypeSF E) : LetRecTypeSF E
-| LRTSF_FunSF (A : StackType) `{IsStackFunc E A} (rest : LetRecTypeSF E) : LetRecTypeSF E.
-
-(* Convert a LetRecTypeSF to a LetRecType by applying all its stack functors *)
-Fixpoint applyLetRecTypeSF E stack (lrtSF : LetRecTypeSF E) : LetRecType :=
-  match lrtSF with
-  | LRTSF_Ret _ R => LRT_Ret (R stack)
-  | LRTSF_Fun _ A rest => LRT_Fun A (fun x => applyLetRecTypeSF E stack (rest x))
-  | LRTSF_FunSF _ A rest => LRT_Fun (A stack) (fun _ => applyLetRecTypeSF E stack rest)
-  end.
-
-(* A RecFrame of stack functor LetRecTypes *)
-Definition RecFrameSF E := list (LetRecTypeSF E).
-
-(* Convert a RecFrameSF to a RecFrame by applying all its LetRecTypeSFs *)
-Fixpoint applyRecFrameSF E stack (frame : RecFrameSF E) : RecFrame :=
-  match frame with
-  | nil => nil
-  | lrtSF :: frame' =>
-      applyLetRecTypeSF E stack lrtSF :: applyRecFrameSF E stack frame'
-  end.
-
-(* Create a multi-way fixed point of a sequence of functions *)
-Definition MultiFixS_SF E Γ frame
-           (bodies : FrameTuple E (frame :: Γ) frame)
-           (call : FrameCall frame) : SpecM E Γ (FrameCallRet frame call) :=
-  mrec_spec (applyFrameTuple E (frame :: Γ) frame bodies) call.
-
-
-
 
 (** Notations in terms of the SpecM combinators **)
 Module SpecMNotations.
@@ -1530,7 +873,7 @@ End interpWithState.
 
 (* Corecursively looks for performances of exceptional effects. If an
    exceptional performance is caught, then `catch` is performed instead. *)
-Program CoFixpoint try_catch {E:EvType} {Γ} {A} {B}
+Program CoFixpoint try_catch {E:EncType} {Γ} {A} {B}
     (is_exceptional : FunStackE E Γ -> option A)
     (catch : A -> SpecM E Γ B) :
     SpecM E Γ B -> SpecM E Γ B :=
